sort/sortcheck.v
@@ -139,18 +139,18 @@ Fixpoint type_check (Γ : context) (t : term) : result term :=
     | _ => Err "Second type argument must be a type"
     end
 
-  | Fst p =>
+  | TFst p =>
       do tyP <- type_check Γ p;
       match tyP with
       | Sigma A B => ret A
       | _ => Err "Fst expects Sigma type"
       end
   
-  | Snd p =>
+  | TSnd p =>
     do tyP <- type_check Γ p;
     match tyP with
     | Sigma A B =>
-        let fst_val := Fst p in
+        let fst_val := TFst p in
         let result_type := subst 0 fst_val B in
         ret (simplify_default result_type)
     | _ => Err "Snd expects Sigma type"
@@ -279,5 +279,1138 @@ Example error_app_non_function :
 reflexivity. Qed.
 
 Example error_fst_non_pair : 
-  type_of (Fst two) = Err "Fst expects Sigma type".
+  type_of (TFst two) = Err "Fst expects Sigma type".
 reflexivity. Qed.
+
+
+
+Definition ctx := list term.
+
+Fixpoint lookup (Γ : ctx) (x : nat) : option term :=
+  match Γ, x with
+  | nil, _ => None
+  | A :: Γ, 0 => Some A
+  | A :: Γ, S n => lookup Γ n
+  end.
+
+Definition conv := multi step.
+
+Inductive infer_type : ctx -> term -> term -> Prop :=
+  | Inf_Var : forall Γ x A,
+      lookup Γ x = Some A ->
+      infer_type Γ (Var x) A
+
+  | Inf_App : forall Γ t u A B,
+      infer_type Γ t (Pi A B) ->
+      check_type Γ u A ->
+      infer_type Γ (App t u) (subst 0 u B)
+
+  | Inf_Star : forall Γ,
+      infer_type Γ Star Star
+
+  | Inf_Nat : forall Γ,
+      infer_type Γ Nat Star
+
+  | Inf_Pi : forall Γ A B,
+      check_type Γ A Star ->
+      check_type (A :: Γ) B Star ->
+      infer_type Γ (Pi A B) Star
+
+  | Inf_Sigma : forall Γ A B,
+      check_type Γ A Star ->
+      check_type (A :: Γ) B Star ->
+      infer_type Γ (Sigma A B) Star
+
+  | Inf_Zero : forall Γ,
+      infer_type Γ Zero Nat
+
+  | Inf_Succ : forall Γ n,
+      infer_type Γ n Nat ->
+      infer_type Γ (Succ n) Nat
+
+  | Inf_Pair : forall Γ A B a b,
+      check_type Γ A Star ->
+      check_type (A :: Γ) B Star ->
+      check_type Γ a A ->
+      check_type Γ b (subst 0 a B) ->
+      infer_type Γ (Pair A B a b) (Sigma A B)
+
+  | Inf_Fst : forall Γ A B p,
+      infer_type Γ p (Sigma A B) ->
+      infer_type Γ (TFst p) A
+
+  | Inf_Snd : forall Γ A B p,
+      infer_type Γ p (Sigma A B) ->
+      infer_type Γ (TSnd p) (subst 0 (TFst p) B)
+
+  | Inf_NatRec : forall Γ P z s n,
+      infer_type Γ P (Pi Nat Star) ->                    (* P : Nat → Type *)
+      check_type Γ z (App P Zero) ->                     (* z : P Zero *)
+      check_type Γ s (Pi Nat (Pi (App P (Var 0))         (* s : Π(n:Nat), P n → P (Succ n) *)
+                                (App P (Succ (Var 0))))) ->
+      infer_type Γ n Nat ->
+      infer_type Γ (NatRec P z s n) (App P n)
+
+  | Inf_Conv : forall Γ t A B,  (* Conversion for inference *)
+      infer_type Γ t A ->
+      check_type Γ B Star ->     (* B must be a valid type *)
+      conv A B ->                (* A and B are convertible *)
+      infer_type Γ t B
+
+with check_type : ctx -> term -> term -> Prop :=
+  | Check_Lam : forall Γ A b B,
+      check_type Γ A Star ->
+      check_type (A :: Γ) b B ->
+      check_type Γ (Lam A b) (Pi A B)
+
+  | Check_Zero : forall Γ,
+      check_type Γ Zero Nat
+
+  | Check_Succ : forall Γ n,
+      check_type Γ n Nat ->
+      check_type Γ (Succ n) Nat
+
+  | Check_Pair : forall Γ A B a b,
+      check_type Γ A Star ->
+      check_type (A :: Γ) B Star ->
+      check_type Γ a A ->
+      check_type Γ b (subst 0 a B) ->
+      check_type Γ (Pair A B a b) (Sigma A B)
+
+  | Check_NatRec : forall Γ P z s n T,
+      check_type Γ P (Pi Nat Star) ->
+      check_type Γ z (App P Zero) ->
+      check_type Γ s (Pi Nat (Pi (App P (Var 0)) 
+                                (App P (Succ (Var 0))))) ->
+      check_type Γ n Nat ->
+      check_type Γ T Star ->
+      conv (App P n) T ->
+      check_type Γ (NatRec P z s n) T
+
+  | Check_Infer : forall Γ t T,
+      infer_type Γ t T ->
+      check_type Γ t T.
+
+Scheme infer_type_mut := Induction for infer_type Sort Prop
+with check_type_mut := Induction for check_type Sort Prop.
+
+Inductive wf_ctx : ctx -> Prop :=
+  | Wf_Empty : wf_ctx nil
+  | Wf_Extend : forall Γ A,
+      wf_ctx Γ ->
+      check_type Γ A Star ->
+      wf_ctx (A :: Γ).
+
+Fixpoint closed (t : term) (k : nat) : Prop :=
+  match t with
+  | Var n    => n < k
+  | Lam A b  => closed A k /\ closed b (S k)
+  | Pi A B   => closed A k /\ closed B (S k)
+  | Sigma A B => closed A k /\ closed B (S k)
+  | Succ n  => closed n k
+  | Pair A B a b => closed A k /\ closed B k /\ closed a k /\ closed b k
+  | TFst p | TSnd p => closed p k
+  | App f a => closed f k /\ closed a k
+  | NatRec P z s n => closed P k /\ closed z k /\ closed s k /\ closed n k
+  | Star | Nat | Zero => True
+  end.
+
+(* canonical atomic types *)
+Inductive atomic_type : term -> Prop :=
+  | at_star : atomic_type Star
+  | at_nat : atomic_type Nat.
+
+(* well-founded types *)
+Inductive wf_type : term -> Prop :=
+  | wf_atomic : forall t,
+      atomic_type t ->
+      wf_type t
+  | wf_pi : forall A B,
+      wf_type A ->                (* domain *)
+      wf_type B ->                (* codomain *)
+      wf_type (Pi A B)
+  | wf_sigma : forall A B,
+      wf_type A ->                (* first component *)
+      wf_type B ->                (* second component *)
+      wf_type (Sigma A B).
+
+Fixpoint is_term (t : term) : bool :=
+  match t with
+  | Var n => true
+  | Zero => true
+  | Succ n => is_term n
+  | Pair A B a b => is_term a && is_term b
+  | Lam A b => is_term b
+  | _ => false
+  end.
+
+(* Non-bidirectional typing without conversion *)
+Inductive has_type2 : ctx -> term -> term -> Prop :=
+  | T_Var : forall Γ x A,
+(*       wf_type A -> *)
+      lookup Γ x = Some A ->
+      has_type2 Γ (Var x) A
+
+  | T_Star : forall Γ,
+      has_type2 Γ Star Star
+
+  | T_Nat : forall Γ,
+      has_type2 Γ Nat Star
+
+  | T_Pi : forall Γ A B,
+      wf_type A ->
+(*       closed A 0 -> *)
+      has_type2 (A :: Γ) B Star ->
+      has_type2 Γ (Pi A B) Star
+
+  | T_Sigma : forall Γ A B,
+      wf_type A ->
+      has_type2 (A :: Γ) B Star ->
+      has_type2 Γ (Sigma A B) Star
+
+  | T_Lam : forall Γ A b B,
+      closed A 0 ->
+      has_type2 (A :: Γ) b B ->
+      has_type2 Γ (Lam A b) (Pi A B)
+
+  | T_App : forall Γ t u A B,
+      wf_type A ->
+      is_term u = true ->
+      closed u 0 ->
+      has_type2 Γ t (Pi A B) ->
+      has_type2 Γ u A ->
+      has_type2 Γ (App t u) (subst 0 u B)
+
+  | T_Zero : forall Γ,
+      has_type2 Γ Zero Nat
+
+  | T_Succ : forall Γ n,
+      has_type2 Γ n Nat ->
+      has_type2 Γ (Succ n) Nat
+
+  | T_Pair : forall Γ A B a b,
+      is_term a = true ->
+      closed a 0 ->
+      has_type2 Γ a A ->
+      has_type2 Γ b (subst 0 a B) ->
+      has_type2 Γ (Pair A B a b) (Sigma A B)
+
+  | T_Fst : forall Γ A B p,
+      wf_type B ->
+      has_type2 Γ p (Sigma A B) ->
+      has_type2 Γ (TFst p) A
+
+  | T_Snd : forall Γ A B p,
+      wf_type A ->
+      is_term (TFst p) = true ->
+      closed p 0 ->
+      has_type2 Γ p (Sigma A B) ->
+      has_type2 Γ (TSnd p) (subst 0 (TFst p) B)
+
+  | T_NatRec : forall Γ P z s n,
+      has_type2 Γ P (Pi Nat Star) ->
+      has_type2 Γ z (App P Zero) ->
+      has_type2 Γ s (Pi Nat (Pi (App P (Var 0)) (App P (Succ (Var 0))))) ->
+      has_type2 Γ n Nat ->
+      has_type2 Γ (NatRec P z s n) (App P n).
+
+Fixpoint zip {A B : Type} (l1 : list A) (l2 : list B) : list (A * B) :=
+  match l1, l2 with
+  | x::xs, y::ys => (x, y) :: zip xs ys
+  | _, _ => []
+  end.
+
+Definition foreach2_ty A B (xs : list A) (ys : list B ) (P : A -> B -> Type) :=
+  fold_right
+    (fun x y => x*y)%type
+    unit%type
+    (map (fun pr:A*B => let (x, y) := pr in P x y) (zip xs ys)).
+
+(** [env_typing] relates a value environment to its typing. It asserts
+    the types (in a [nil] environment) of each of a series of values. *)
+Definition env_typing Vs Ts :=
+  ((List.length Vs = List.length Ts) *
+  foreach2_ty _ _ Vs Ts (fun x y => (has_type2 nil x y (* /\ is_term x = true *) /\ wf_type y)))%type.
+
+(** [env_typing_env] also relates a value environment to its typing. It asserts
+    the types (in a given environment) of each of a series of values. *)
+Definition env_typing_env env Vs Ts :=
+  ((List.length Vs = List.length Ts) *
+  foreach2_ty _ _ Vs Ts (fun x y => (has_type2 env x y (* /\ is_term x = true *) /\ wf_type y)))%type.
+
+Hint Unfold env_typing.
+
+(** [env_typing_env] environments can be extended, one term-type pair at a time. *)
+Lemma env_typing_intro:
+  forall env V Vs T Ts,
+    wf_type T ->
+    has_type2 env V T ->
+    env_typing_env env (Vs) (Ts) ->
+    env_typing_env env (V::Vs) (T::Ts).
+Proof.
+ intros.
+ unfold env_typing_env in *.
+ unfold foreach2_ty in *.
+ simpl in *.
+ intuition.
+ 
+Qed.
+
+Require Import Coq.Arith.Peano_dec.
+
+Require Import Coq.Arith.PeanoNat.
+
+Fixpoint subst_env (k : nat) (vs : list term) (t : term) {struct t} : term :=
+  match t with
+  | Var x =>
+      if Nat.leb k x then
+        match nth_error vs (x - k) with
+        | Some v => lift 0 k v
+        | None => Var x
+        end
+      else Var x
+  | Star => Star
+  | Nat => Nat
+  | Pi A B =>
+      Pi (subst_env k vs A)
+         (subst_env (S k) (map (lift 0 1) vs) B)
+  | Sigma A B =>
+      Sigma (subst_env k vs A)
+            (subst_env (S k) (map (lift 0 1) vs) B)
+  | Lam A b =>
+      Lam (subst_env k vs A)
+          (subst_env (S k) (map (lift 0 1) vs) b)
+  | App t1 t2 =>
+      App (subst_env k vs t1) (subst_env k vs t2)
+  | Zero => Zero
+  | Succ n => Succ (subst_env k vs n)
+  | Pair A B a b =>
+      Pair (subst_env k vs A) (subst_env k vs B)
+           (subst_env k vs a) (subst_env k vs b)
+  | TFst p => TFst (subst_env k vs p)
+  | TSnd p => TSnd (subst_env k vs p)
+  | NatRec P z s n =>
+      NatRec (subst_env k vs P)
+             (subst_env k vs z)
+             (subst_env k vs s)
+             (subst_env k vs n)
+  end.
+
+Lemma wftS: forall T c,
+  wf_type T -> has_type2 c T Star.
+Proof. intro T.
+       induction T; intros.
+       3:{ inversion H.
+           - subst.
+             inversion H0.
+           - subst. 
+             constructor. easy.
+             apply IHT2. easy.
+         }
+       11:{ inversion H.
+            subst.
+            inversion H0.
+          }
+       9:{ inversion H.
+           subst.
+           inversion H0.
+         }
+       9:{ inversion H. subst. inversion H0. }
+       6:{ inversion H. subst.
+           inversion H0.
+         }
+       - constructor.
+       - constructor.
+       - constructor.
+         inversion H. subst. inversion H0.
+         subst. easy.
+         apply IHT2. 
+         inversion H. subst. inversion H0.
+         subst. easy.
+       - inversion H.
+         subst. easy.
+       - inversion H.
+         subst. easy.
+       - inversion H.
+         subst. easy.
+       - inversion H.
+         subst. easy.
+       - inversion H.
+         subst. easy.
+Qed.
+
+Lemma liftterm: forall A n k, is_term A = true -> is_term (lift n k A) = true.
+Proof. intro A.
+       induction A; intros.
+       3:{ simpl in H. easy. }
+       10:{ simpl. inversion H. rewrite IHA2. easy. easy. }
+       9:{ simpl. destruct (n <? k); easy. }
+       6:{ simpl. inversion H.
+           rewrite IHA3, IHA4. easy.
+           apply Bool.andb_true_iff in H1. easy.
+           apply Bool.andb_true_iff in H1. easy.
+          }
+       8:{ simpl in H. easy. }
+       - simpl in H. easy.
+       - easy.
+       - easy.
+       - easy.
+       - simpl in H. simpl.
+         apply IHA. easy.
+       - easy.
+       - easy.
+       - easy.
+Qed.
+
+Lemma wfsubstR: forall B A n, is_term A = true -> wf_type B -> wf_type (subst n A B).
+Proof. intro B.
+       induction B; intros.
+       3:{ simpl in H.
+           inversion H0.
+           subst. inversion H1.
+           subst.
+           simpl.
+           apply wf_pi. 
+           apply IHB1. easy. easy.
+           apply IHB2. apply liftterm. easy. easy.
+         }
+       10:{ simpl in H.
+           inversion H0.
+           subst. inversion H1.
+          }
+       10:{ simpl in H.
+            inversion H0.
+             subst. inversion H1.
+          }
+        9:{ simpl in H0.
+            inversion H0. inversion H1.
+          }
+        6:{ inversion H0. subst.
+            inversion H1.
+          }
+        - simpl. easy.
+        - simpl. easy.
+        - simpl. inversion H0.
+          subst. easy.
+          subst. simpl.
+          apply wf_sigma.
+          apply IHB1; easy.
+          apply IHB2. apply liftterm. easy. easy.
+        - easy.
+        - simpl. inversion H0.
+          subst. easy.
+        - simpl. inversion H0.
+          subst. easy.
+        - simpl. inversion H0.
+          subst. easy.
+        - simpl. inversion H0.
+          subst. easy.
+Qed.
+
+Lemma wfsubstL: forall B A n, is_term A = true -> wf_type (subst n A B) -> wf_type B.
+Proof. intro B.
+       induction B; intros.
+       3:{ simpl in H.
+           inversion H0.
+           subst. inversion H1.
+           subst.
+           apply wf_pi. apply IHB1 with (n:= n) (A := A). easy. easy. 
+           apply IHB2 with (A := (lift 1 0 A)) (n := S n). 
+           apply liftterm. easy. easy.
+         }
+       10:{ simpl in H.
+           inversion H0.
+           subst. inversion H1.
+          }
+       10:{ simpl in H.
+            inversion H0.
+             subst. inversion H1.
+          }
+        9:{ simpl in H0.
+            case_eq(n ?= n0); intros. rewrite H1 in H0. rewrite lift_0 in H0.
+            - inversion H0. subst.
+              inversion H2.
+              subst. easy.
+              subst. easy.
+              subst. easy.
+              subst. easy.
+            - rewrite H1 in H0.
+              easy.
+            - rewrite H1 in H0.
+              inversion H0. subst. easy.
+          }
+          6:{ inversion H0. subst.
+              inversion H1.
+            }
+          - easy.
+          - easy.
+          - simpl in H0.
+            inversion H0.
+            subst. easy.
+            subst.
+            apply wf_sigma.
+            apply IHB1 with (A := A) (n := n); easy.
+            apply IHB2 with (A := (lift 1 0 A)) (n := S n).
+            apply liftterm. easy. easy.
+          - easy.
+          - simpl in H0. inversion H0. subst. easy.
+          - simpl in H0. inversion H0. subst. easy.
+          - simpl in H0. inversion H0. subst. easy.
+          - simpl in H0. inversion H0. subst. easy.
+Qed.
+
+Require Import List.
+
+Lemma shift_nonfree_noop :
+  forall M n k env T,
+    wf_type T ->
+    length env <= k ->
+    has_type2 env M T -> lift n k M = M.
+Proof.
+ intro M.
+ induction M; simpl; intros.
+ 3:{ simpl.
+     inversion H1. subst.
+     rewrite IHM1 with (env := env) (T := Star).
+     rewrite IHM2 with (env := (M1 :: env)) (T := Star). easy.
+     simpl. constructor. constructor.
+     simpl. lia.
+     easy. easy. easy.
+     apply wftS with (c := env) in H5. easy.
+    }
+  9: { inversion H1. subst.
+      case_eq(n <? k); intros.
+      + easy.
+      + admit.
+    }
+  10:{ simpl.
+       inversion H1. subst.
+       rewrite IHM1 with (env := env) (T := (Pi A B)).
+       rewrite IHM2 with (env := env) (T := A).
+       easy. easy. easy. easy.
+       apply wf_pi. easy. apply wfsubstL in H. easy.
+       easy.
+       easy. easy.
+    }
+  6:{ simpl. inversion H1. subst.
+      inversion H. subst. easy.
+      subst.
+      rewrite IHM1 with (env := env) (T := Star).
+      rewrite IHM2 with (env := env) (T := Star).
+      rewrite IHM3 with (env := env) (T := M1).
+      rewrite IHM4 with (env := env) (T := (subst 0 M3 M2)).
+      easy.
+      apply wfsubstR. easy. easy.
+      easy. easy.
+      easy.
+      easy.
+      easy. constructor. constructor.
+      easy.
+      apply wftS. easy. constructor. constructor.
+      easy.
+      apply wftS. easy.
+     }
+  - easy.
+  - easy.
+  - simpl. 
+    inversion H1. subst.
+    rewrite IHM1 with (env := env) (T := Star).
+    rewrite IHM2 with (env := (M1 :: env)) (T := Star).
+    easy. easy. simpl. lia. easy. easy. easy.
+    apply wftS with (c := env) in H5. easy.
+  - easy.
+  - simpl. inversion H1. subst.
+    rewrite IHM with (env := env) (T := Nat).
+    easy. easy. easy. easy.
+  - simpl. inversion H1. subst.
+    rewrite IHM with (env := env) (T := (Sigma T B)).
+    easy.
+    apply wf_sigma. easy. easy.
+    easy. easy.
+  - simpl. inversion H1. subst.
+    rewrite IHM with (env := env) (T := (Sigma A B)).
+    easy.
+    apply wf_sigma. easy. easy.
+    easy. easy.
+  - simpl. 
+    inversion H1. subst.
+    rewrite IHM1 with (env := env) (T := Star).
+    rewrite IHM2 with (env := (M1 :: env)) (T := B).
+    easy. inversion H. subst. easy. subst. easy. simpl. lia.
+    easy. constructor. constructor. easy.
+    inversion H. easy.
+    apply wftS with (c := env) in H4. easy.
+  - simpl.
+    inversion H1. subst.
+    inversion H. subst. easy.
+Admitted.
+
+
+Lemma env_typing_shift_noop :
+  forall Vs env,
+    env_typing Vs env ->
+    forall n k, map (lift n k) Vs = Vs.
+Proof.
+ intro Vs.
+ induction Vs; simpl; intros env H; auto.
+ intros n k.
+ inversion H as [len tps].
+ case_eq env; intros.
+ + subst. easy.
+ + subst.
+ unfold foreach2_ty in tps.
+ simpl in tps.
+ f_equal.
+  inversion tps.
+  eapply shift_nonfree_noop with (T := t) (env := nil); eauto. easy. simpl.
+  
+  simpl; lia. easy.
+ rewrite IHVs with (env := l); auto.
+ unfold env_typing.
+ split. inversion len. easy.
+ unfold foreach2_ty.
+ destruct tps.
+ easy.
+Qed.
+
+Lemma shift_preserves_typing:
+  forall M k n env1 env2 env env' T,
+    wf_type T ->
+    env1 ++ env2 = env ->
+    k = length env1 ->
+    n = length env' ->
+    has_type2 env M T -> 
+    has_type2 (env1++env'++env2) (lift n k M) T.
+Proof. intro M.
+       induction M; intros.
+       11: { simpl.
+             inversion H3. subst. simpl in *.
+             rewrite shift_nonfree_noop with (env := env1) (T := Star).
+             apply T_Lam. easy.
+             specialize (IHM2  (S (Datatypes.length env1)) (Datatypes.length env')
+              (M1 :: env1) env2 ((M1 :: env1) ++ env2) env' B).
+             simpl in IHM2. apply IHM2. inversion H. subst. easy. subst. easy.
+             easy.
+             easy.
+             easy. easy. constructor. constructor. easy.
+             inversion H. subst. easy. subst.
+             apply wftS with (c := env1) in H2. easy.
+          }
+        10: { inversion H3. subst.
+              inversion H.
+              - subst. inversion H0. 
+                + subst.
+                  simpl.
+                  case_eq( n <? Datatypes.length env1); intros.
+                  ++ apply T_Var. admit.
+                  ++ apply T_Var. admit.
+                + subst. simpl.
+                  case_eq( n <? Datatypes.length env1); intros.
+                  ++ apply T_Var. admit.
+                  ++ apply T_Var. admit.
+              - subst. simpl.
+                case_eq( n <? Datatypes.length env1); intros.
+                + constructor. admit.
+                + constructor. admit.
+              - subst. simpl.
+                case_eq( n <? Datatypes.length env1); intros.
+                + apply T_Var. admit.
+                + apply T_Var. admit.
+             }
+        3: { simpl.
+             inversion H3. subst.
+             rewrite shift_nonfree_noop with (env := env1) (T := Star).
+             constructor.
+             easy.
+            specialize (IHM2  (S (Datatypes.length env1)) (Datatypes.length env')
+              (M1 :: env1) env2 ((M1 :: env1) ++ env2) env' Star).
+            simpl in IHM2. apply IHM2. easy. easy. easy. easy. easy. easy. easy.
+            apply wftS with (c := env1) in H7. easy.
+          }
+        9: { inversion H3. subst. simpl in *.
+             assert((lift (Datatypes.length env') (Datatypes.length env1) M2) = M2) by admit.
+             rewrite H0.
+             apply T_App with (A := A) (B := B). easy. easy. easy.
+             apply IHM1 with (env := env1 ++ env2 ).
+             apply wf_pi. easy.
+             apply wfsubstL with (A := M2) (n := 0). easy. easy.
+             easy.
+             easy. easy. easy.
+             rewrite <- H0.
+             apply IHM2 with (env := env1 ++ env2 ). easy. easy. easy.
+             easy. easy.
+           }
+        - simpl.
+          inversion H3. constructor.
+        - simpl. inversion H3. constructor.
+        - simpl. inversion H3. subst.
+          rewrite shift_nonfree_noop with (env := env1) (T := Star).
+          apply T_Sigma. easy.
+          specialize (IHM2  (S (Datatypes.length env1)) (Datatypes.length env')
+           (M1 :: env1) env2 ((M1 :: env1) ++ env2) env' Star).
+          simpl in IHM2. apply IHM2. inversion H. subst. easy. easy.
+          easy.
+          easy.
+          easy. easy. easy.
+          apply wftS with (c := env1) in H7. easy.
+        - inversion H3. subst. simpl.
+          constructor.
+        - inversion H3. subst. simpl.
+          constructor.
+          apply IHM with (env := (env1 ++ env2)).
+          easy. easy. easy. easy. easy.
+        - inversion H3. subst. simpl.
+          setoid_rewrite shift_nonfree_noop with (env := env1) (T := Star) at 2.
+          setoid_rewrite shift_nonfree_noop with (env := env1) (T := Star) at 1.
+          apply T_Pair.
+          admit.
+          admit.
+          apply IHM3 with (env := (env1 ++ env2)).
+          inversion H. easy. easy. easy. easy. easy.
+          easy.
+          simpl.
+          apply IHM4 with (env := (env1 ++ env2) ).
+          admit.
+          easy.
+          easy. easy. 
+          admit. 
+          constructor. constructor. easy.
+          admit.
+          constructor. constructor. easy.
+          admit.
+        - inversion H3. subst.
+          simpl.
+          apply T_Fst with (B := B). easy.
+          apply IHM with (env := (env1 ++ env2)).
+          apply wf_sigma. easy. easy.
+          easy. easy. easy. easy.
+        - inversion H3. subst.
+          simpl.
+          assert((lift (Datatypes.length env') (Datatypes.length env1) M) = M) by admit.
+          rewrite H0.
+          apply T_Snd with (A := A). easy. easy. easy.
+          rewrite <- H0.
+          apply IHM with (env := (env1 ++ env2)).
+          apply wf_sigma. easy. easy.
+          easy. easy. easy. easy.
+        - subst.
+          inversion H3. subst. simpl.
+          inversion H. subst. easy.
+Admitted.
+
+Lemma substitution :
+  forall M N A B Γ1 Γ2,
+    wf_type B ->
+    has_type2 (Γ1 ++ A :: Γ2) M B ->
+    has_type2 Γ2 N A ->
+    has_type2 (Γ1 ++ Γ2) (subst (length Γ2) N M) B.
+Admitted.
+
+(* (* Inductive *)
+
+From MMaps Require Import MMaps.
+
+Require Import Coq.FSets.FMapAVL.
+Require Import Coq.Structures.OrderedTypeEx.
+
+
+Module M := MMaps.RBT.Make(Nat).
+Module MF := MMaps.Facts.Properties Nat M.
+
+Definition ctx: Type := M.t term.
+
+(* Typing relation *)
+Inductive has_type : ctx -> term -> term -> Prop :=
+  | T_Star : forall Γ,
+      has_type Γ Star Star
+  | T_Nat : forall Γ,
+      has_type Γ Nat Star
+  | T_Var : forall Γ x T,
+      M.find x Γ = Some T ->
+      has_type Γ (Var x) T
+  | T_Pi : forall Γ G A B k,
+      has_type Γ A Star ->
+      G = (M.add k A Γ) ->
+      has_type G B Star ->
+      has_type Γ (Pi A B) Star
+  | T_Lam : forall Γ G A b B k,
+      G = (M.add k A Γ) ->
+      has_type G B Star ->
+      has_type Γ (Lam A b) (Pi A B)
+  | T_App : forall Γ f a A B,
+      has_type Γ f (Pi A B) ->
+      has_type Γ a A ->
+      has_type Γ (App f a) B
+  | T_Sigma : forall Γ G A B k,
+      has_type Γ A Star ->
+      G = (M.add k A Γ) ->
+      has_type G B Star ->
+      has_type Γ (Sigma A B) Star
+  | T_Pair : forall Γ A B a b,
+      has_type Γ a A ->
+      has_type Γ b B ->
+      has_type Γ (Pair A B a b) (Sigma A B)
+  | T_Fst : forall Γ p A B,
+      has_type Γ p (Sigma A B) ->
+      has_type Γ (TFst p) A
+  | T_Snd : forall Γ p A B,
+      has_type Γ p (Sigma A B) ->
+      has_type Γ (TSnd p) B
+  | T_Zero : forall Γ,
+      has_type Γ Zero Nat
+  | T_Succ : forall Γ n,
+      has_type Γ n Nat ->
+      has_type Γ (Succ n) Nat
+  | T_NatRec : forall Γ P z s n k,
+      has_type Γ n Nat ->
+      has_type Γ z Nat ->
+      has_type (M.add k Nat Γ) s (Pi Nat (Pi Nat Nat)) ->
+      has_type Γ (NatRec P z s n) Nat.
+
+Definition lift_ctx (d k: nat) (Γ : ctx) : ctx :=
+  M.map (fun T => lift d k T) Γ.
+
+Lemma lift_preserves_typing_map :
+  forall Γ t T d k,
+    has_type Γ t T ->
+    has_type (lift_ctx d k Γ) (lift d k t) (lift d k T).
+Proof.
+  intros Γ t T d k Hty.
+  revert d k.
+  induction Hty; intros.
+  4:{ simpl.
+      apply T_Pi with (G := M.add k (lift d k0 A) (lift_ctx d k0 Γ)) (k := k). simpl in *. easy.
+      easy.
+      simpl in *.
+      simpl in *.
+      
+   constructor. 
+
+
+Example type_addI : has_type (M.empty) add (Pi Nat (Pi Nat Nat)).
+Proof.
+  unfold add.
+  apply T_Lam with (k := 0).                    (* λ m *)
+  apply T_Lam with (k := 1).                    (* λ n *)
+  apply T_NatRec with (k := 2).
+  - apply T_Var. simpl. reflexivity.  (* Var 1 : Nat *)
+  - apply T_Var. simpl. reflexivity.  (* Var 0 : Nat *)
+  - apply T_Lam with (k := 3).                    (* λ m *)
+    apply T_Lam with (k := 4).          (* step function s *)
+    apply T_Succ. apply T_Var. simpl; reflexivity.
+Qed.
+
+Example type_add2 : has_type (extend (extend (extend (extend (extend (M.empty) 0 Nat) 1 Nat) 2 Nat) 3 Nat) 4 Nat) add
+  (Pi Nat (Pi Nat Nat)).
+Proof.
+  unfold add.
+  apply T_Lam with (k := 0).                    (* λ m *)
+  apply T_Lam with (k := 1).                    (* λ n *)
+  apply T_NatRec with (k := 2).
+  - apply T_Var. simpl. reflexivity.  (* Var 1 : Nat *)
+  - apply T_Var. simpl. reflexivity.  (* Var 0 : Nat *)
+  - apply T_Lam with (k := 3).                    (* λ m *)
+    apply T_Lam with (k := 4).          (* step function s *)
+    apply T_Succ. apply T_Var. simpl; reflexivity.
+Qed.
+
+
+Example type_mult : has_type (M.empty) mult (Pi Nat (Pi Nat Nat)).
+Proof.
+  unfold mult.
+  (* mult = Lam Nat (Lam Nat (NatRec ...)) *)
+  (* Step 1: type the outer Lam *)
+  apply T_Lam with (k := 0). 
+  (* Context now: [Nat] *)
+  (* Step 2: type the inner Lam *)
+  apply T_Lam with (k := 1).
+  (* Context now: [Nat; Nat] *)
+  (* Step 3: type NatRec *)
+  apply T_NatRec with (k := 2).
+  - (* n : Var 1, which is the first argument in context, type Nat *)
+    apply T_Var. simpl. reflexivity.
+  - (* base case z = Zero : Nat *)
+    apply T_Zero.
+  - (* step function s = Lam Nat (Lam Nat (App (App add (Var 0)) (Var 2))) *)
+    apply T_Lam with (k := 3).
+    (* Context now: [Nat; Nat; Nat] *)
+    apply T_Lam with (k := 4).
+    (* Context now: [Nat; Nat; Nat; Nat] *)
+    (* Body: App (App add (Var 0)) (Var 2) *)
+    apply T_App with (A := Nat).
+    + apply T_App with (A := Nat).
+      apply type_add2.
+      apply T_Var. simpl. reflexivity.
+    + (* argument Var 2 : Nat *)
+      apply T_Var. simpl. reflexivity.
+Qed.
+
+ *)
+(* (* List-based context *)
+Definition ctx := list term.
+
+(* Lookup a variable by de Bruijn index *)
+Definition lookup (Γ : ctx) (n : nat) : option term :=
+  nth_error Γ n.
+
+(* Extend context under a binder *)
+Definition extend (Γ : ctx) (T : term) : ctx := T :: Γ. *)
+
+(* Inductive has_type : ctx -> term -> term -> Prop :=
+  | T_Star : forall Γ, has_type Γ Star Star
+  | T_Nat : forall Γ, has_type Γ Nat Star
+  | T_Var : forall Γ x T, lookup Γ x = Some T -> has_type Γ (Var x) T
+  | T_Pi : forall Γ A B, has_type Γ A Star -> has_type (A :: Γ) B Star -> has_type Γ (Pi A B) Star
+  | T_Lam : forall Γ A b B, has_type (A :: Γ) b B -> has_type Γ (Lam A b) (Pi A B)
+  | T_App : forall Γ f a A B, has_type Γ f (Pi A B) -> has_type Γ a A -> has_type Γ (App f a) B
+  | T_Sigma : forall Γ A B, has_type Γ A Star -> has_type (A :: Γ) B Star -> has_type Γ (Sigma A B) Star
+  | T_Pair : forall Γ A B a b, has_type Γ a A -> has_type Γ b B -> has_type Γ (Pair A B a b) (Sigma A B)
+  | T_Fst : forall Γ p A B, has_type Γ p (Sigma A B) -> has_type Γ (TFst p) A
+  | T_Snd : forall Γ p A B, has_type Γ p (Sigma A B) -> has_type Γ (TSnd p) B
+  | T_Zero : forall Γ, has_type Γ Zero Nat
+  | T_Succ : forall Γ n, has_type Γ n Nat -> has_type Γ (Succ n) Nat
+  | T_NatRec : forall Γ P z s n, has_type Γ n Nat -> has_type Γ z Nat -> has_type (Nat :: Γ) s (Pi Nat (Pi Nat Nat)) -> has_type Γ (NatRec P z s n) Nat.
+
+Lemma lift_id_below_all :
+  forall t d k,
+    (forall n, occurs_inb n t = true -> n < k) ->
+    lift d k t = t.
+Proof. intro t.
+       induction t; intros.
+        10:{
+        simpl in *.
+        specialize(H n).
+        assert((n =? n) = true).
+        { rewrite Nat.eqb_refl. easy. }
+        apply H in H0.
+        apply Nat.ltb_lt in H0. rewrite H0. easy.
+        }
+       - easy.
+       - easy.
+       - simpl.
+         rewrite IHt1, IHt2. easy.
+         intros. simpl in H.
+         specialize(H n).
+         assert(occurs_inb n t1 || occurs_inb n t2 = true).
+         { rewrite H0. lia. }
+         apply H in H1. lia.
+         intros. simpl in H.
+         specialize(H n).
+         assert(occurs_inb n t1 || occurs_inb n t2 = true).
+         { rewrite H0. lia. }
+         apply H in H1. lia.
+Admitted.
+
+Lemma lift_under_extend_correct :
+  forall t d k,
+    (forall n, occurs_inb n t = true -> n < k) ->
+    lift d (k+1) t = lift d k (lift 1 k t).
+Admitted.
+
+Lemma lookup_extend_eq :
+  forall Γ T n,
+    lookup (T :: Γ) (S n) = lookup Γ n.
+Proof.
+  intros Γ T n.
+  simpl.
+  (* nth_error (T :: Γ) n = nth_error Γ (n - 1) if n > 0 *)
+  destruct n.
+  - easy.
+  - easy.
+Qed.
+
+Lemma ctx_eqe: forall x Γ Δ A T,
+  (forall (x : nat) (T' : term), lookup Γ x = Some T' -> lookup Δ x = Some T') ->
+  lookup (A :: Γ) x = Some T ->
+  lookup (A :: Δ) x = Some T.
+Proof. intro x.
+       induction x; intros.
+       - simpl in *. easy.
+       - simpl in *. apply H. easy.
+Qed.
+
+Lemma weakening : forall Γ Δ t T,
+  has_type Γ t T ->
+  (forall x T', lookup Γ x = Some T' -> lookup Δ x = Some T') ->
+  has_type Δ t T.
+Proof.
+  intros Γ Δ t T Htyp Hlook.
+  revert Δ Hlook.
+  induction Htyp; intros.
+  4:{
+  constructor. 
+  apply IHHtyp1. easy.
+  apply IHHtyp2. intros.
+  apply ctx_eqe with ( Γ :=  Γ). easy.
+  easy.
+  }
+  3:{ 
+  constructor.
+  apply Hlook. easy.
+
+  }
+  
+  constructor.
+  constructor.
+
+  constructor. 
+  apply IHHtyp.
+  intros.
+  apply ctx_eqe with ( Γ :=  Γ). easy.
+  easy.
+  
+  apply T_App with (A := A).
+  apply IHHtyp1. easy.
+  apply IHHtyp2. easy.
+
+  constructor. 
+  apply IHHtyp1. easy.
+  apply IHHtyp2. intros.
+  apply ctx_eqe with ( Γ :=  Γ). easy.
+  easy.
+
+  constructor.
+  apply IHHtyp1. easy.
+  apply IHHtyp2. intros.
+  apply Hlook. easy.
+
+  apply T_Fst with (B:=B).
+  apply IHHtyp.
+  intros. apply Hlook. easy.
+
+  apply T_Snd with (A:=A).
+  apply IHHtyp.
+  intros. apply Hlook. easy.
+  
+  constructor.
+  constructor.
+  apply IHHtyp. easy.
+  
+  constructor.
+  apply IHHtyp1. easy.
+  apply IHHtyp2. easy.
+  apply IHHtyp3. intros.
+
+  
+  apply ctx_eqe with ( Γ :=  Γ). easy.
+  easy.
+Qed. *)
+
+Lemma lift_closed_gen :
+  forall t k d,
+    closed t k ->   (* t has no free variables after depth k *)
+    lift d k t = t.
+Proof.
+  intros t.
+  induction t; intros.
+  10:{ simpl. inversion H. 
+       simpl in H. subst.
+       assert(n <? S n = true).
+       { apply Nat.ltb_lt. lia. }
+       rewrite H0.
+       easy.
+       subst. simpl in H. 
+       assert(n <? S m = true).
+       { apply Nat.ltb_lt. lia. }
+       rewrite H1.
+       easy.
+  }
+  admit.
+  admit.
+  - (* Pi A B *)
+    destruct H as [HA HB].
+    simpl. rewrite IHt2.
+    rewrite IHt1. easy. easy. easy.
+Admitted.
+
+Lemma lift_closed_id :
+  forall t d,
+    closed t 0 ->   (* t has no free variables after depth k *)
+    lift d 0 t = t.
+Proof. intros. rewrite lift_closed_gen.
+       easy. easy.
+Qed.
+
+Lemma closed_weaken : forall t k k',
+  k <= k' ->
+  closed t k ->
+  closed t k'.
+Proof. intro t.
+       induction t; intros.
+       3:{ simpl in *.
+           split. apply IHt1 with (k := k). easy. easy.
+           apply IHt2 with (k := S k). lia. easy.
+         }
+       9:{ simpl in *. lia. }
+Admitted.
+
+Lemma closed_lift : forall t k d,
+  closed t k ->
+  closed (lift d k t) (k + d).
+Proof. intro t.
+       induction t; intros.
+       3:{ simpl.
+           split. apply IHt1. simpl in H. easy.
+           apply IHt2. simpl in H. easy.
+         }
+       9:{ simpl.
+           simpl in H.
+           apply Nat.ltb_lt in H. rewrite H.
+           simpl.
+           apply Nat.ltb_lt in H. lia.
+         }
+Admitted.
+
+Lemma lift_closed_general :
+  forall t d k k',
+    closed t k -> k <= k' -> closed (lift d k t) (k' + d).
+Proof. intros.
+       apply closed_lift with (d := d) in H.
+       apply closed_weaken with (k := k + d). lia.
+       easy.
+Qed.
+
+(* Lemma subst_closed_shift :
+  forall t s j d,
+    closed t (S j + d) ->
+    closed s 0 ->
+    closed (subst (j + d) (lift d 0 s) t) (j + d).
+Proof. intro t.
+       induction t; intros.
+       3:{ simpl. split.
+           apply IHt1.
+(*            apply closed_weaken with (k := j); try lia. *)
+           simpl in H. easy.
+           easy.
+           simpl.
+           rewrite lift_lift.
+           specialize(IHt2 s j (S d)).
+           simpl in IHt2. 
+           assert((j + S d) = S (j + d)) by lia.
+           rewrite H1 in IHt2.
+           assert(1 + d = S d) by lia.
+           rewrite H2.
+           apply IHt2. simpl in H. easy. easy.
+         }
+        9:{ simpl.
+            destruct (n ?= j + d) eqn:E.
+            simpl. rewrite lift_0. simpl.
+            apply lift_closed_general. easy.
+            lia. inversion H. subst.
+            admit.
+            subst.
+            inversion H. subst. admit.
+            subst.
+            apply closed_weaken with (k := S (j + d)).
+            + simpl.
+              
+              rewrite E.
+              simpl in *.
+               (* variable does not match: stays Var n *)
+              apply Nat.eqb_neq in E.
+              lia.
+           }
+Admitted. *)
+
+
+
